\subsection{Formula explanation}
\label{appendix:formula_explanation}

% String literals
\newcommand{\mse}{\text{MSE}(\hat{\pi}^{\star})}
\newcommand{\bias}{\text{Bias}_{\pi}}
\newcommand{\variance}{\text{Var}_\pi}
% Operations
\newcommand{\sumovert}{\sum_{t=1}^{T}}
\newcommand{\meanovert}{\frac{1}{T}\sum_{t=1}^{T}}
% Population parameter and inflation measure
\newcommand{\hatpi}{\hat{\pi}^{\star}}
\newcommand{\barhatpi}{\overline{\hat{\pi}^{\star}}}
\newcommand{\barpi}{\overline{\pi}}
\newcommand{\err}{e}
% Standard errors of parameter and estimator
\newcommand{\spi}{s_{\pi}}
\newcommand{\shatpi}{s_{\hatpi}}
\newcommand{\corr}{r^{\star}}


Consider the error time series $\err_t = \hatpi_t - \pi_t$ for the inflation measure $\hatpi$. Then, $\bias = \meanovert\err_t = \meanovert\hatpi_t - \meanovert\pi_t = \barhatpi-\barpi$. 
First, we show in \ref{eq:mse_is_square_error_plus_bias} that $\mse = \bias^2 + \variance$, where $\variance=\meanovert(\err_t-\bias)^2$ represents the variance of prediction error. This is the classical bias-variance decomposition of the mean square error. 

\begin{equation}
    \begin{aligned}
        \mse & = \meanovert (\hatpi_t - \pi_t)^2\\
        ~ & = \meanovert \left[ (\err_t - \bias) + \bias \right]^2 \\
        ~ & = \meanovert\bias^2 + 2\,\bias\,\meanovert(\err_t-\bias) + \meanovert(\err_t-\bias)^2  \\
        ~ & = \bias^2 + \underbrace{2\,\bias\left(\meanovert\err_t - \meanovert\bias\right)}_{=0} + \meanovert(\err_t-\bias)^2\\
        ~ & = \bias^2 + \variance
    \end{aligned}
    \label{eq:mse_is_square_error_plus_bias}
\end{equation}
